code/Yazi.LZ77.fst
@@ -27,7 +27,11 @@ open Yazi.Stream.Types
 open Yazi.Stream.State
 
 [@
-  (CPrologue "#include <string.h>
+  (CPrologue "#ifdef _MSC_VER
+#include <intrin.h>
+#endif
+
+#include <string.h>
 static inline uint32_t lz77_hash(uint16_t h_bits, const unsigned char *buf) {
   uint32_t n;
   memcpy(&n, buf, sizeof(n));
@@ -439,3 +443,322 @@ let fill_window ss ctx ls next_in wrap block_start block_data =
   in
   ST.pop_frame ();
   res
+
+[@ (CEpilogue "#include \"Yazi_LZ77_String.inc\"")]
+assume val ctz_compare:
+     len: U32.t
+  -> s: B.buffer U8.t
+  -> m: B.buffer U8.t
+  -> i: U32.t
+  -> ST.Stack U32.t
+  (requires fun h -> S.ctz_compare_pre h len s m i)
+  (ensures fun h0 res h1 -> S.ctz_compare_post h0 res h1 len s m i)
+
+[@ CInline ]
+let rec match_iteration_1 (s m: B.buffer U8.t) (i tail: U32.t):
+  ST.Stack U32.t
+  (requires fun h -> S.string_compare_ite_pre h s m i tail /\ U32.v tail < 4)
+  (ensures fun h0 len h1 -> S.string_compare_ite_post h0 len h1 s m i tail) =
+  let open U32 in
+  if i <^ tail then
+    if s.(i) = m.(i) then
+      match_iteration_1 s m (i +^ 1ul) tail
+    else
+      i
+  else
+    i
+
+[@ CInline ]
+let rec match_iteration_8 (s m: B.buffer U8.t) (i tail: U32.t):
+  ST.Stack U32.t
+  (requires fun h ->
+    S.string_compare_ite_pre h s m i tail /\
+    (U32.v tail - U32.v i) % 8 == 0)
+  (ensures fun h0 len h1 -> S.string_compare_ite_post h0 len h1 s m i tail)
+  (decreases (U32.v tail - U32.v i)) =
+  let open U32 in
+  if U32.lt i tail then begin
+    let len = ctz_compare 8ul s m i in
+    if len = 8ul then
+      match_iteration_8 s m (i +^ len) tail
+    else
+      i +^ len
+  end else
+    i
+
+#set-options "--z3rlimit 1024 --fuel 0 --ifuel 0"
+[@ CInline ]
+let match_iteration (s m: B.buffer U8.t) (tail: U32.t):
+  ST.Stack U32.t
+  (requires fun h ->
+    B.live h s /\ B.live h m /\
+    B.length s <= B.length m /\
+    U32.v tail <= B.length s /\
+    U32.v tail <= S.max_match)
+  (ensures fun h0 len h1 ->
+    let s' = B.as_seq h0 s in
+    let m' = B.as_seq h0 m in
+    let len' = U32.v len in
+    let tail' = U32.v tail in
+    B.modifies B.loc_none h0 h1 /\
+    len' <= tail' /\
+    (len' < tail' ==> s'.[len'] <> m'.[len']) /\
+    (forall (j: nat{j < len'}). s'.[j] == m'.[j])) =
+  let open U32 in
+  let r1 = tail %^ 4ul in
+  let l1 = if r1 = 0ul then 0ul else match_iteration_1 s m 0ul r1 in
+  let t4 = tail -^ r1 in
+  if l1 = r1 && t4 >^ 0ul then
+    let r4 = t4 %^ 8ul in
+    if r4 = 0ul then
+      match_iteration_8 s m l1 tail
+    else
+      let l4 = ctz_compare 4ul s m l1 in
+      if l4 = 4ul then begin
+        match_iteration_8 s m (l1 +^ 4ul) tail
+      end else
+        l1 +^ l4
+  else
+    l1
+
+[@ (CEpilogue "#define Yazi_LZ77_fast_compare(s1, s2, len) memcmp(s1, s2, (size_t)len)")]
+assume val fast_compare: 
+    s1: B.buffer U8.t
+  -> s2: B.buffer U8.t
+  -> len: U32.t
+  -> ST.Stack I32.t
+  (requires fun h ->
+    B.live h s1 /\ B.live h s2 /\
+    B.length s1 >= U32.v len /\ B.length s2 >= U32.v len)
+  (ensures fun h0 res h1 ->
+    let s1' = B.as_seq h0 s1 in
+    let s2' = B.as_seq h0 s2 in
+    B.modifies B.loc_none h0 h1 /\
+    (I32.v res == 0 <==> (forall (i: nat{i < U32.v len}). s1'.[i] == s2'.[i])))
+
+unfold let slow_match_pre_cond
+  (h: HS.mem)
+  (ctx: lz77_context_p)
+  (s: lz77_state_t)
+  (scan_end limit chain_length cur_match: U32.t) =
+  let open U32 in
+  let s' = B.as_seq h s in
+  let ctx' = B.get h (CB.as_mbuf ctx) 0 in
+  CFlags.fastest == false /\
+  S.longest_match_pre h ctx s cur_match /\
+  v scan_end + S.min_match <= S.window_end s' /\
+  S.strstart s' <= v scan_end /\
+  (S.strstart s' >= v ctx'.w_size ==> v limit == S.strstart s' - v ctx'.w_size) /\
+  (S.strstart s' < v ctx'.w_size ==> v limit == 0) /\
+  v chain_length >= 1
+
+[@ CInline ]
+#set-options "--z3rlimit 4096 --fuel 0 --ifuel 0 --z3seed 13"
+let rec search_hash_chain
+  (ctx: lz77_context_p)
+  (s: lz77_state_t)
+  (scan_end limit chain_length i: U32.t):
+  ST.Stack (U32.t & U32.t & bool)
+  (requires fun h -> slow_match_pre_cond h ctx s scan_end limit chain_length i)
+  (ensures fun h0 res h1 ->
+    let open U32 in
+    let (cur_match, chain_length', cont) = res in
+    let s' = B.as_seq h1 s in
+    let w = B.as_seq h1 (B.get h1 (CB.as_mbuf ctx) 0).window in
+    let strstart = S.strstart s' in
+    B.modifies B.loc_none h0 h1 /\
+    (cont == true ==>
+      v cur_match < strstart /\
+      (forall (k: nat{k < S.min_match}).
+        w.[v cur_match + k] == w.[strstart + k]) /\
+      U32.v chain_length' <= U32.v chain_length))
+  (decreases U32.v chain_length) =
+  let open U32 in
+  let h0 = Ghost.hide (ST.get ()) in
+  let ctx' = Ghost.hide (B.get h0 (CB.as_mbuf ctx) 0) in
+  let window = (CB.index ctx 0ul).window in
+  let strstart = get_strstart s in
+  let s1 = B.sub window strstart min_match in
+  let s2 = B.sub window i min_match in
+  let e1 = B.sub window scan_end min_match in
+  let e2 = B.sub window (scan_end -^ strstart +^ i) min_match in
+  let c1 = fast_compare s1 s2 min_match in
+  let c2 = fast_compare e1 e2 min_match in
+  if c1 = 0l && c2 = 0l then begin
+    let w = Ghost.hide (B.as_seq h0 window) in
+    let d = Ghost.hide (v strstart - v i) in
+    let s1' = Ghost.hide (B.as_seq h0 (B.gsub window strstart min_match)) in
+    let s2' = Ghost.hide (B.as_seq h0 (B.gsub window i min_match)) in
+    let strstart' = Ghost.hide (U32.v strstart) in
+    assert(forall (j: nat{j < S.min_match}).
+      s1'.[j] == s2'.[j] /\ s1'.[j] == w.[strstart' + j] /\ s2'.[j] == w.[v i + j]);
+    assert(forall (j: nat{j < S.min_match}). {:pattern (w.[v i + j]); (w.[strstart' + j])}
+      w.[v i + j] == w.[strstart' + j]);
+    (i, chain_length, true)
+  end else if chain_length >^ 1ul then begin
+    let prev = (CB.index ctx 0ul).prev in
+    let w_mask = (CB.index ctx 0ul).w_mask in
+    [@inline_let] let w_mask' = Cast.uint16_to_uint32 w_mask in
+    UInt.logand_mask #32 (v i) (U16.v ctx'.w_bits);
+    let i' = prev.(i &^ w_mask') in
+    let i'' = Cast.uint16_to_uint32 i' in
+    if i'' >^ limit then
+      search_hash_chain ctx s scan_end limit (chain_length -^ 1ul) i''
+    else
+      (0ul, 0ul, false)
+  end else
+    (0ul, 0ul, false)
+
+[@ CInline ]
+let rec do_longest_match_slow
+  (ctx: lz77_context_p)
+  (s: lz77_state_t)
+  (nice_match scan_end limit chain_length cur_match best_len: U32.t):
+  ST.Stack (U32.t & U32.t)
+  (requires fun h ->
+    let open U32 in
+    let ctx' = B.get h (CB.as_mbuf ctx) 0 in
+    let s' = B.as_seq h s in
+    let w = B.as_seq h ctx'.window in
+    slow_match_pre_cond h ctx s scan_end limit chain_length cur_match /\
+    (S.nice_match s' < S.lookahead s' ==> v nice_match == S.nice_match s') /\
+    (S.nice_match s' >= S.lookahead s' ==> v nice_match == S.lookahead s') /\
+    (v best_len > 0 ==>
+      (v best_len >= S.min_match /\
+      v cur_match < S.strstart s' /\
+      S.strstart s' + v best_len <= S.window_end s' /\
+      (forall (i: nat{i < v best_len}). w.[v cur_match + i] == w.[S.strstart s' + i]))))
+  (ensures fun h0 res h1 ->
+    let open U32 in
+    let ctx' = B.get h1 (CB.as_mbuf ctx) 0 in
+    let s' = B.as_seq h1 s in
+    let w = B.as_seq h1 ctx'.window in
+    let (bl, cm) = res in
+    B.modifies B.loc_none h0 h1 /\
+    v bl >= v best_len /\
+    (v bl >= S.min_match ==>
+      v cm < S.strstart s' /\
+      S.strstart s' + v bl <= S.window_end s' /\
+      (forall (i: nat{i < v bl}). w.[v cm + i] == w.[S.strstart s' + i])))
+  (decreases U32.v chain_length) =
+  let open U32 in
+  if nice_match <^ best_len then
+    let (cm, cl, cont) = search_hash_chain ctx s scan_end limit chain_length cur_match in
+    if cont then begin
+      let w_bits = (CB.index ctx 0ul).w_bits in
+      let window = (CB.index ctx 0ul).window in
+      let strstart = get_strstart s in
+      let lookahead = get_lookahead s in
+      let max_lookahead = if w_bits = 8us then 256ul else 258ul in
+      let max_offset = 
+        (if lookahead <^ max_lookahead then lookahead else max_lookahead) -^ min_match in
+      let sbuf = B.sub window (strstart +^ min_match) (Ghost.hide max_offset) in
+      let mbuf = B.sub window (cm +^ min_match) (Ghost.hide max_offset) in
+      let l' = match_iteration sbuf mbuf max_offset in
+      let l = min_match +^ l' in
+
+      let h = Ghost.hide (ST.get ()) in
+      let w = Ghost.hide (B.as_seq h window) in
+      assert(forall (i: nat{S.min_match <= i /\ i < S.min_match + v l'}).
+        (B.as_seq h sbuf).[i - S.min_match] == (B.as_seq h mbuf).[i - S.min_match] /\
+        (B.as_seq h sbuf).[i - S.min_match] == w.[v strstart + i] /\
+        (B.as_seq h mbuf).[i - S.min_match] == w.[v cm + i]);
+      assert(forall (i:nat{i < v l}).
+        {:pattern (w.[v cm + i]); (w.[v strstart + i])}
+        w.[v cm + i] == w.[v strstart + i]);
+
+      if l >^ best_len then
+        if cl >^ 1ul && cm >^ 0ul then
+          do_longest_match_slow
+            ctx s nice_match (strstart +^ l -^ 4ul) limit (cl -^ 1ul) cm l
+        else
+          (l, cm)
+      else
+        if cl >^ 1ul then
+          do_longest_match_slow
+            ctx s nice_match scan_end limit (cl -^ 1ul) cur_match best_len
+        else
+          (best_len, cur_match)
+    end else
+      (best_len, cur_match)
+  else
+    (best_len, cur_match)
+
+[@ CInline ]
+let do_longest_match_fast (ctx: lz77_context_p) (s: lz77_state_t) (cur_match: U32.t):
+  ST.Stack U32.t
+  (requires fun h -> S.longest_match_pre h ctx s cur_match)
+  (ensures fun h0 res h1 ->
+    let open U32 in
+    let ctx' = B.get h1 (CB.as_mbuf ctx) 0 in
+    let s' = B.as_seq h1 s in
+    let w = B.as_seq h1 ctx'.window in
+    B.modifies B.loc_none h0 h1 /\
+    (v res >= S.min_match ==>
+      S.strstart s' + v res <= S.window_end s' /\
+      (forall (i: nat{i < v res}). w.[v cur_match + i] == w.[S.strstart s' + i]))) =
+  let open U32 in
+  let w_bits = (CB.index ctx 0ul).w_bits in
+  let window = (CB.index ctx 0ul).window in
+  let strstart = get_strstart s in
+  let lookahead = get_lookahead s in
+  
+  let max_lookahead = if w_bits = 8us then 256ul else 258ul in
+  let max_offset = if lookahead <^ max_lookahead then lookahead else max_lookahead in
+
+  let sbuf = B.sub window strstart (Ghost.hide max_offset) in
+  let mbuf = B.sub window cur_match (Ghost.hide max_offset) in
+
+  let h = Ghost.hide (ST.get ()) in
+  let w = Ghost.hide (B.as_seq h window) in
+  
+  let l = match_iteration sbuf mbuf max_offset in
+  assert(forall (i: nat{i < v l}).
+    (B.as_seq h sbuf).[i] == (B.as_seq h mbuf).[i] /\
+    (B.as_seq h sbuf).[i] == w.[v strstart + i] /\
+    (B.as_seq h mbuf).[i] == w.[v cur_match + i]);
+  assert(forall (i:nat{i < v l}).
+    {:pattern (w.[v cur_match + i]); (w.[v strstart + i])}
+    w.[v cur_match + i] == w.[v strstart + i]);
+  l
+
+let longest_match ctx s cur_match =
+  let open U32 in
+  let strstart = get_strstart s in
+  let prev_length = get_prev_length s in
+  let w_size = (CB.index ctx 0ul).w_size in
+  let limit = if strstart >^ w_size then strstart -^ w_size else 0ul in
+
+  let h0 = Ghost.hide (ST.get ()) in
+  let ctx' = Ghost.hide (B.get h0 (CB.as_mbuf ctx) 0) in
+
+  if CFlags.fastest then
+    let len = do_longest_match_fast ctx s cur_match in
+    if len <=^ prev_length then
+      min_match -^ 1ul
+    else begin
+      set_match_start (U16.v ctx'.w_bits) (v ctx'.w_size) s cur_match;
+      len
+    end
+  else
+    let nm = get_nice_match s in
+    let lookahead = get_lookahead s in
+    let nice_match = if nm <^ lookahead then nm else lookahead in
+    let limit = if strstart >^ w_size then strstart -^ w_size else 0ul in
+    let good_match = get_good_match s in
+    let mcl = get_max_chain_length s in
+    let chain_length = if prev_length >=^ good_match then mcl <<^ 2ul else mcl in
+    let se1 = strstart +^ prev_length -^ (min_match -^ 1ul) in
+    let se2 = strstart +^ lookahead -^ min_match in
+    let scan_end = if se1 >^ se2 then se2 else se1 in
+    if chain_length >^ 0ul then
+      let (bl, cm) = do_longest_match_slow
+        ctx s nice_match scan_end
+        limit chain_length cur_match 0ul in
+      if bl >^ prev_length then begin
+        set_match_start (U16.v ctx'.w_bits) (v ctx'.w_size) s cm;
+        bl
+      end else
+        min_match -^ 1ul
+    else
+      min_match -^ 1ul
