specs/Spec.LZ77.fst
@@ -51,6 +51,7 @@ unfold let context_valid (h: HS.mem) (ctx: lz77_context_p) =
   let open U16 in
   CB.length ctx == 1 /\
   (let c = B.get h (CB.as_mbuf ctx) 0 in
+
   is_window_bits (v c.w_bits) /\
   is_window_mask (v c.w_bits) (v c.w_mask) /\
   is_window_size (v c.w_bits) (U32.v c.w_size) /\
@@ -62,6 +63,7 @@ unfold let context_valid (h: HS.mem) (ctx: lz77_context_p) =
   is_hash_mask (v c.h_bits) (v c.h_mask) /\
   U32.v c.window_size - min_match + 1 > U32.v c.w_size /\
   B.length c.head == U32.v c.h_size /\
+  
   CB.live h ctx /\ B.live h c.prev /\ B.live h c.window /\ B.live h c.head /\ B.live h c.prev /\
   B.disjoint c.window c.prev /\ B.disjoint c.window c.head /\ B.disjoint c.prev c.head /\
   B.frameOf c.window == B.frameOf c.prev /\ B.frameOf c.prev == B.frameOf c.head /\
@@ -226,7 +228,7 @@ let hash_chain_valid
   (CFlags.fastest == false ==> prev_valid h ctx h_range slided) /\
   head_valid h ctx h_range slided
 
-type lz77_state = s:Seq.seq U32.t{Seq.length s == 7}
+type lz77_state = s:Seq.seq U32.t{Seq.length s == 13}
 
 unfold let match_length (s: lz77_state) = U32.v s.[0]
 unfold let match_start (s: lz77_state) = U32.v s.[1]
@@ -235,6 +237,13 @@ unfold let prev_length (s: lz77_state) = U32.v s.[3]
 unfold let strstart (s: lz77_state) = U32.v s.[4]
 unfold let lookahead (s: lz77_state) = U32.v s.[5]
 unfold let insert (s: lz77_state) = U32.v s.[6]
+unfold let level (s: lz77_state) = U32.v s.[7]
+unfold let strategy (s: lz77_state) = U32.v s.[8]
+unfold let max_chain_length (s: lz77_state) = U32.v s.[9]
+unfold let max_lazy_match (s: lz77_state) = U32.v s.[10]
+unfold let good_match (s: lz77_state) = U32.v s.[11]
+unfold let nice_match (s: lz77_state) = U32.v s.[12]
+
 unfold let window_end (s: lz77_state) = strstart s + lookahead s
 unfold let hash_end (s: lz77_state) = strstart s - insert s
 unfold let max_hash_end (s: lz77_state) = window_end s - min_match + 1
@@ -246,6 +255,25 @@ unfold let prev_length_unchange (s0 s1: lz77_state) = prev_length s0 == prev_len
 unfold let strstart_unchange (s0 s1: lz77_state) = strstart s0 == strstart s1
 unfold let lookahead_unchange (s0 s1: lz77_state) = lookahead s0 == lookahead s1
 unfold let insert_unchange (s0 s1: lz77_state) = insert s0 == insert s1
+
+unfold let level_unchange (s0 s1: lz77_state) = level s0 == level s1
+unfold let strategy_unchange (s0 s1: lz77_state) = strategy s0 == strategy s1
+unfold let max_chain_length_unchange (s0 s1: lz77_state) =
+  max_chain_length s0 == max_chain_length s1
+unfold let max_lazy_match_unchange (s0 s1: lz77_state) =
+  max_lazy_match s0 == max_lazy_match s1
+unfold let good_match_unchange (s0 s1: lz77_state) =
+  good_match s0 == good_match s1
+unfold let nice_match_unchange (s0 s1: lz77_state) =
+  nice_match s0 == nice_match s1
+
+unfold let deflate_params_unchange (s0 s1: lz77_state) =
+  level_unchange s0 s1 /\
+  strategy_unchange s0 s1 /\
+  max_chain_length_unchange s0 s1 /\
+  max_lazy_match_unchange s0 s1 /\
+  good_match_unchange s0 s1 /\
+  nice_match_unchange s0 s1
 
 // This condition should hold in all acases for all LZ77 states.
 unfold let state_valid (h: HS.mem) (ctx: lz77_context_p) (s: lz77_state_t) =
@@ -260,9 +288,16 @@ unfold let state_valid (h: HS.mem) (ctx: lz77_context_p) (s: lz77_state_t) =
   insert s' <= strstart s' /\
   hash_end s' + min_match - 1 <= window_end s' /\
   match_length s' <= min_match /\
-  prev_length s' <= min_match /\
+  prev_length s' <= max_match /\
   match_start s' <= 2 * U32.v ctx'.w_size - min_match /\
-  prev_match s' <= 2 * U32.v ctx'.w_size - min_match)
+  prev_match s' < 2 * U32.v ctx'.w_size - min_match /\
+  level s' <= 9 /\ strategy s' <= 4 /\ max_chain_length s' <= U32.v ctx'.w_size /\
+  max_lazy_match s' <= max_match /\ good_match s' <= max_match /\ nice_match s' <= max_match /\
+  
+  max_chain_length s' <= 4096 /\
+  max_lazy_match s' <= max_match /\
+  good_match s' <= max_match /\
+  nice_match s' <= max_match)
 
 unfold let window_valid
   (h: HS.mem)
@@ -392,6 +427,7 @@ private unfold let slide_window_buf_post'
   match_length_unchange s0 s1 /\
   prev_match_unchange s0 s1 /\ prev_length_unchange s0 s1 /\
   lookahead_unchange s0 s1 /\ insert_unchange s0 s1 /\
+  deflate_params_unchange s0 s1 /\
   
   strstart s0 - U32.v ctx'.w_size == strstart s1 /\
   match_start s0 - U32.v ctx'.w_size == match_start s1 /\
@@ -524,7 +560,8 @@ unfold let do_fill_window_post
     match_start_unchange ls0 ls1 /\
     match_length_unchange ls0 ls1 /\
     prev_match_unchange ls0 ls1 /\
-    prev_length_unchange ls0 ls1
+    prev_length_unchange ls0 ls1 /\
+    deflate_params_unchange ls0 ls1
 
 let fill_window_pre
   (h: HS.mem)
@@ -607,27 +644,28 @@ unfold let fill_window_post
     match_length_unchange ls0 ls1 /\
     prev_match_unchange ls0 ls1 /\
     prev_length_unchange ls0 ls1 /\
+    deflate_params_unchange ls0 ls1 /\
     strstart ls1 < U32.v ctx'.w_size /\
     window_valid h1 ctx ls block_data' /\
     SS.avail_out_unchange ss0 ss1 /\ SS.total_out_unchange ss0 ss1 /\
     block_start1 >= -8454144
 
-unfold let ctz_compare_pre (h: HS.mem) (len: nat) (s m: B.buffer U8.t) (i: U32.t) =
-  (len == 4 \/ len == 8) /\
+unfold let ctz_compare_pre (h: HS.mem) (len: U32.t) (s m: B.buffer U8.t) (i: U32.t) =
+  (U32.v len == 4 \/ U32.v len == 8) /\
   B.live h s /\ B.live h m /\
   B.length m >= B.length s /\
-  U32.v i + len <= B.length s /\
+  U32.v i + U32.v len <= B.length s /\
   (forall (j: nat{j < U32.v i}). (B.as_seq h s).[j] == (B.as_seq h m).[j])
 
 let ctz_compare_post
-  (h0: HS.mem) (res: U32.t) (h1: HS.mem) (len: nat) (s m: B.buffer U8.t) (i: U32.t) =
+  (h0: HS.mem) (res: U32.t) (h1: HS.mem) (len: U32.t) (s m: B.buffer U8.t) (i: U32.t) =
     let s' = B.as_seq h0 s in
     let m' = B.as_seq h0 m in
     let res' = U32.v res in
     let i' = U32.v i in
     ctz_compare_pre h0 len s m i /\
     B.modifies B.loc_none h0 h1 /\
-    res' <= len /\ (res' == len \/ s'.[i' + res'] <> m'.[i' + res']) /\
+    res' <= U32.v len /\ (res' == U32.v len \/ s'.[i' + res'] <> m'.[i' + res']) /\
     (forall (j: nat{j < i' + res'}). s'.[j] == m'.[j])
 
 unfold let string_compare_ite_pre (h: HS.mem) (s m: B.buffer U8.t) (i tail: U32.t) =
@@ -638,7 +676,7 @@ unfold let string_compare_ite_pre (h: HS.mem) (s m: B.buffer U8.t) (i tail: U32.
   B.live h s /\ B.live h m /\ B.length s <= B.length m /\
   tail' <= max_match /\
   tail' <= B.length s /\ i' <= tail' /\
-  i' <= tail' /\ (forall (j: nat{j < U32.v i}). s'.[j] == m'.[j])
+  i' <= tail' /\ (forall (j: nat{j < U32.v i}). {:pattern (s'.[j]); (m'.[j])} s'.[j] == m'.[j])
 
 unfold let string_compare_ite_post
   (h0: HS.mem) (len: U32.t) (h1: HS.mem) (s m: B.buffer U8.t) (i tail: U32.t) =
@@ -649,11 +687,41 @@ unfold let string_compare_ite_post
     B.modifies B.loc_none h0 h1 /\
     U32.v tail <= B.length s /\ B.length s <= B.length m /\
     len' <= tail' /\ (len' == tail' \/ s'.[len'] <> m'.[len']) /\
-    (forall (j: nat{j < len'}). s'.[j] == m'.[j])
+    (forall (j: nat{j < len'}). {:pattern (s'.[j]); (m'.[j])} s'.[j] == m'.[j])
 
 unfold let match_ready (h: HS.mem) (ctx: lz77_context_p) (s: lz77_state_t) =
   let s' = B.as_seq h s in
+  let ctx' = B.get h (CB.as_mbuf ctx) 0 in
   state_valid h ctx s /\
   insert s' == 0 /\
-  lookahead s' >= min_lookahead (B.get h (CB.as_mbuf ctx) 0) /\
+  lookahead s' >= min_match /\
+  strstart s' > 0 /\
+  strstart s' <= U32.v ctx'.window_size - max_match /\
+  prev_length s' >= min_match - 1 /\
   hash_chain_valid h ctx (U32.uint_to_t (hash_end s')) false
+
+unfold let longest_match_pre
+  (h: HS.mem) (ctx: lz77_context_p) (s: lz77_state_t) (cur_match: U32.t) =
+  let s' = B.as_seq h s in
+  match_ready h ctx s /\ 0 < U32.v cur_match /\ U32.v cur_match < strstart s'
+  
+unfold let longest_match_post
+  (h0: HS.mem)
+  (len: U32.t)
+  (h1: HS.mem)
+  (ctx: lz77_context_p)
+  (s: lz77_state_t)
+  (cur_match: U32.t) =
+  let open U32 in
+  let s' = B.as_seq h1 s in
+  let w = B.as_seq h0 (B.get h0 (CB.as_mbuf ctx) 0).window in
+  longest_match_pre h0 ctx s cur_match /\
+  state_valid h1 ctx s /\
+  (v len < min_match ==> B.modifies B.loc_none h0 h1) /\
+  (v len >= min_match ==>
+    B.modifies (B.loc_buffer s) h0 h1 /\
+    LB.unchange_except h0 h1 s 1 /\
+    prev_length s' < v len /\
+    match_start s' < strstart s' /\
+    strstart s' + v len <= window_end s' /\
+    (forall (i: nat{i < v len}). w.[match_start s' + i] == w.[strstart s' + i]))
