Makefile
@@ -152,7 +152,7 @@ KRML=$(KREMLIN_HOME)/krml
 # easily turn this file into a .h, use -add-include '"Impl_Bignum_Intrinsics.h"'
 # and pass -static-header Impl.Bignum.Intrinsics as described in the
 # documentation.
-HAND_WRITTEN_C_FILES = code/c/Yazi_Allocator.h code/c/Yazi_Z_Stream_Fields.inc code/c/Yazi_Adler32_Z.inc
+HAND_WRITTEN_C_FILES = code/c/Yazi_Allocator.h code/c/Yazi_Z_Stream_Fields.inc code/c/Yazi_Adler32_Z.inc code/c/Yazi_LZ77_String.inc
 
 # This is now the preferred and recommended way to compile C code with KreMLin.
 #
